end of day 18/06/19

formal/Contexts.thy
@@ -11,9 +11,11 @@ theory Contexts
 begin
 
 definition can_take :: "transition \<Rightarrow> inputs \<Rightarrow> registers \<Rightarrow> bool" where
-  "can_take t i r = apply_guards (Guard t) (join_ir i r)"
+  "can_take t i r = (length i = Arity t \<and> apply_guards (Guard t) (join_ir i r))"
 
-lemma medial_subset: "set (Guard t') \<subseteq> set (Guard t) \<Longrightarrow> can_take t i r \<longrightarrow> can_take t' i r"
+lemma medial_subset: "length i = Arity t \<Longrightarrow>
+                      Arity t = Arity t' \<Longrightarrow>
+                      set (Guard t') \<subseteq> set (Guard t) \<Longrightarrow> can_take t i r \<longrightarrow> can_take t' i r"
   by (simp add: can_take_def apply_guards_subset)
 
 definition d2r :: "datastate \<Rightarrow> registers" where
@@ -22,8 +24,8 @@ definition d2r :: "datastate \<Rightarrow> registers" where
 lemma d2r_keeps_regs_same [simp]: "d2r c r = c (R r)"
   by (simp add: d2r_def)
 
-definition posterior :: "transition \<Rightarrow> datastate \<Rightarrow> registers option" where
-  "posterior t d = (if apply_guards (Guard t) d then Some (apply_updates (Updates t) d (d2r d)) else None)"
+definition posterior :: "transition \<Rightarrow> inputs \<Rightarrow> registers \<Rightarrow> registers option" where
+  "posterior t i r = (if can_take t i r then Some (apply_updates (Updates t) (join_ir i r) r) else None)"
 
 definition r2d :: "registers \<Rightarrow> datastate" where
   "r2d regs = (\<lambda>i. case i of R r \<Rightarrow> regs r | _ \<Rightarrow> None)"
@@ -32,26 +34,27 @@ definition subsumes :: "transition \<Rightarrow> registers \<Rightarrow> transit
   "subsumes t2 r t1 = (Label t1 = Label t2 \<and> Arity t1 = Arity t2 \<and>
                        (\<forall>i. can_take t1 i r \<longrightarrow> can_take t2 i r) \<and>
                        (\<forall>i. can_take t1 i r \<longrightarrow> apply_outputs (Outputs t1) (join_ir i r) = apply_outputs (Outputs t2) (join_ir i r)) \<and>
-                       (\<forall>p1 p2 i. posterior t2 (join_ir i r) = Some p2 \<and> posterior t1 (join_ir i r) = Some p1 \<longrightarrow> (\<forall>P r'. (p1 r' = None) \<or> (P (p2 r') \<longrightarrow> P (p1 r')))) \<and>
-                       (\<forall>p1 p2 i. posterior t2 (join_ir i r) = Some p2 \<and> posterior t1 (join_ir i r) = Some p1 \<longrightarrow> (\<forall>r. p1 r \<noteq> None \<longrightarrow>  p2 r \<noteq> None))
+                       (\<forall>p1 p2 i. posterior t2 i r = Some p2 \<and> posterior t1 i r = Some p1 \<longrightarrow> (\<forall>P r'. (p1 r' = None) \<or> (P (p2 r') \<longrightarrow> P (p1 r')))) \<and>
+                       (\<forall>p1 p2 i. posterior t2 i r = Some p2 \<and> posterior t1 i r = Some p1 \<longrightarrow> (\<forall>r. p1 r \<noteq> None \<longrightarrow>  p2 r \<noteq> None))
                       )"
 
 lemma subsumption: 
   "(Label t1 = Label t2 \<and> Arity t1 = Arity t2) \<Longrightarrow>
    (\<forall>i. can_take t1 i r \<longrightarrow> can_take t2 i r) \<Longrightarrow>
    (\<forall>i. can_take t1 i r \<longrightarrow> apply_outputs (Outputs t1) (join_ir i r) = apply_outputs (Outputs t2) (join_ir i r)) \<Longrightarrow>
-   (\<forall>p1 p2 i. posterior t2 (join_ir i r) = Some p2 \<and> posterior t1 (join_ir i r) = Some p1 \<longrightarrow> (\<forall>P r. (p1 r = None) \<or> (P (p2 r) \<longrightarrow> P (p1 r)))) \<Longrightarrow>
-   (\<forall>p1 p2 i. posterior t2 (join_ir i r) = Some p2 \<and> posterior t1 (join_ir i r) = Some p1 \<longrightarrow> (\<forall>r. p1 r \<noteq> None \<longrightarrow>  p2 r \<noteq> None)) \<Longrightarrow>
+   (\<forall>p1 p2 i. posterior t2 i r = Some p2 \<and> posterior t1 i r = Some p1 \<longrightarrow> (\<forall>P r'. (p1 r' = None) \<or> (P (p2 r') \<longrightarrow> P (p1 r')))) \<Longrightarrow>
+   (\<forall>p1 p2 i. posterior t2 i r = Some p2 \<and> posterior t1 i r = Some p1 \<longrightarrow> (\<forall>r. p1 r \<noteq> None \<longrightarrow>  p2 r \<noteq> None)) \<Longrightarrow>
    subsumes t2 r t1"
   by (simp add: subsumes_def)
 
-lemma inconsistent_updates: "\<exists>p1 p2. (\<exists>i. posterior t2 (join_ir i r) = Some p2 \<and> posterior t1 (join_ir i r) = Some p1) \<and> (\<exists>r. (\<exists>y. p1 r = Some y) \<and> p2 r = None) \<Longrightarrow>
+lemma bad_guards: "\<exists>i. can_take t1 i r \<and> \<not> can_take t2 i r \<Longrightarrow> \<not> subsumes t2 r t1"
+  by (simp add: subsumes_def)
+
+lemma inconsistent_updates: "\<exists>p1 p2. (\<exists>i. posterior t2 i r = Some p2 \<and> posterior t1 i r = Some p1) \<and> (\<exists>r. (\<exists>y. p1 r = Some y) \<and> p2 r = None) \<Longrightarrow>
  \<not> subsumes t2 r t1"
   by (simp add: subsumes_def)
 
-lemma inconsistent_updates2: "\<exists>p1 p2.
-       (\<exists>i. posterior t2 (join_ir i r) = Some p2 \<and> posterior t1 (join_ir i r) = Some p1) \<and>
-       (\<exists>P r. P (p2 r) \<and> (\<exists>y. p1 r = Some y) \<and> \<not> P (p1 r)) \<Longrightarrow>
+lemma inconsistent_updates2: "\<exists>p1 p2. (\<exists>i. posterior t2 i r = Some p2 \<and> posterior t1 i r = Some p1) \<and> (\<exists>P r'. P (p2 r') \<and> (\<exists>y. p1 r' = Some y) \<and> \<not> P (p1 r')) \<Longrightarrow>
  \<not> subsumes t2 r t1"
   by (simp add: subsumes_def)
 
@@ -114,4 +117,6 @@ qed
 lemma accepts_trace_gives_context: "accepts_trace e p \<Longrightarrow> (\<exists>c. anterior_context e p = Some c)"
   using accepts_gives_context by auto
 
+lemma accepts_trace_anterior_not_none: "accepts_trace e p \<Longrightarrow> anterior_context e p \<noteq> None"
+  using accepts_trace_gives_context by blast
 end
