formal/inference/heuristics/Store_Reuse.thy
@@ -170,7 +170,7 @@ lemmas remove_guard_add_update_preserves = remove_guard_add_update_preserves_lab
                                            remove_guard_add_update_preserves_outputs
 
 definition is_generalisation_of :: "transition \<Rightarrow> transition \<Rightarrow> nat \<Rightarrow> nat \<Rightarrow> bool" where
-  "is_generalisation_of t' t i r = (t' = remove_guard_add_update t i r \<and> (\<exists>v. gexp.Eq (V (I i)) (L v) \<in> set (Guard t)) \<and> r \<notin> set (map fst (Updates t)))"
+  "is_generalisation_of t' t i r = (t' = remove_guard_add_update t i r \<and> i \<le> Arity t \<and> i > 0 \<and> (\<exists>v. gexp.Eq (V (I i)) (L v) \<in> set (Guard t)) \<and> r \<notin> set (map fst (Updates t)))"
 
 lemma generalise_output_preserves_label: "Label (generalise_output t r p) = Label t"
   by (simp add: generalise_output_def)
